progress i think

sat.dfy
@@ -33,7 +33,7 @@ datatype Expression =
     }
     
     ghost function height() : (h: int)
-        ensures h >= 0
+        ensures h >= 1
     {
         match this {
             case Constant(b) => 1
@@ -445,119 +445,220 @@ datatype Expression =
         assert Or(a,b).eval(vs) == And(Or(a,bc1), Or(a,bc2)).eval(vs);
     }
 
-    function DistributeEquivalent2Abitrary(vs: map<Variable, bool>, a: Expression, b: Expression, c: Expression, d: Expression, e: Expression, f: Expression) : (out: Expression)
-        requires a.Valid() && b.Valid() && c.Valid() && d.Valid() && e.Valid() && f.Valid()
-        requires a == And(c,d)
-        requires b == And(e,f)
-        ensures out == And(And(Or(c,e),Or(d,e)),And(Or(c,f),Or(d,f)))
-        ensures Or(a,b).eval(vs) == out.eval(vs)
+    // function DistributeEquivalent2Abitrary(vs: map<Variable, bool>, a: Expression, b: Expression, c: Expression, d: Expression, e: Expression, f: Expression) : (out: Expression)
+    //     requires a.Valid() && b.Valid() && c.Valid() && d.Valid() && e.Valid() && f.Valid()
+    //     requires a == And(c,d)
+    //     requires b == And(e,f)
+    //     ensures out == And(And(Or(c,e),Or(d,e)),And(Or(c,f),Or(d,f)))
+    //     ensures Or(a,b).eval(vs) == out.eval(vs)
+    // {
+    //     assert Or(a,b).eval(vs) == Or(a,And(e,f)).eval(vs);
+    //     DistributeEquivalent1(a, And(e,f), e, f);
+    //     assert Or(a,b).eval(vs) == And(
+    //         Or(a,e), 
+    //         Or(a,f)
+    //     ).eval(vs);
+
+    //     assert Or(a,e).eval(vs) == Or(And(c,d),e).eval(vs);
+    //     DistributeEquivalent1(e, And(c,d), c, d);
+    //     assert Or(a,e).eval(vs) == And(Or(c,e),Or(d,e)).eval(vs);
+
+    //     assert Or(a,f).eval(vs) == Or(And(c,d),f).eval(vs);
+    //     DistributeEquivalent1(f, And(c,d), c, d);
+    //     assert Or(a,f).eval(vs) == And(Or(c,f),Or(d,f)).eval(vs);
+
+    //     var out := And(
+    //         And(Or(c,e),Or(d,e)),
+    //         And(Or(c,f),Or(d,f))
+    //     );
+    //     assert Or(a,b).eval(vs) == out.eval(vs);
+    //     out
+    // }
+
+    // lemma DistributeEquivalent2(a: Expression, b: Expression, c: Expression, d: Expression, e: Expression, f: Expression)
+    //     requires a.Valid() && b.Valid() && c.Valid() && d.Valid() && e.Valid() && f.Valid()
+    //     requires a == And(c,d)
+    //     requires b == And(e,f)
+    //     ensures Or(a,b).equivalent(And(And(Or(c,e),Or(d,e)),And(Or(c,f),Or(d,f))))
+    // {
+    //     assert forall m: map<Variable, bool> :: true ==> 
+    //         (
+    //             ghost var vs: map<Variable, bool> :| vs == m;
+    //             var out := DistributeEquivalent2Abitrary(vs, a, b, c, d, e, f);
+    //             assert Or(a,b).eval(vs) == And(And(Or(c,e),Or(d,e)),And(Or(c,f),Or(d,f))).eval(vs);
+    //             Or(a,b).eval(m) == out.eval(m)
+    //         );
+    // }
+
+    
+
+    ghost function top_two_or_and_heights() : (h: (int, int))
+        requires this.Valid()
+        ensures this.height() >= h.0 >= h.1 >= 0
+        ensures forall i :: i in this.children() ==> h.0 >= i.top_two_or_and_heights().0
+        ensures forall i :: i in this.children() ==>
+            h.0 > i.top_two_or_and_heights().0 || h.1 >= i.top_two_or_and_heights().1
     {
-        assert Or(a,b).eval(vs) == Or(a,And(e,f)).eval(vs);
-        DistributeEquivalent1(a, And(e,f), e, f);
-        assert Or(a,b).eval(vs) == And(
-            Or(a,e), 
-            Or(a,f)
-        ).eval(vs);
-
-        assert Or(a,e).eval(vs) == Or(And(c,d),e).eval(vs);
-        DistributeEquivalent1(e, And(c,d), c, d);
-        assert Or(a,e).eval(vs) == And(Or(c,e),Or(d,e)).eval(vs);
-
-        assert Or(a,f).eval(vs) == Or(And(c,d),f).eval(vs);
-        DistributeEquivalent1(f, And(c,d), c, d);
-        assert Or(a,f).eval(vs) == And(Or(c,f),Or(d,f)).eval(vs);
-
-        var out := And(
-            And(Or(c,e),Or(d,e)),
-            And(Or(c,f),Or(d,f))
-        );
-        assert Or(a,b).eval(vs) == out.eval(vs);
-        out
+        match this {
+            case Constant(b) => (0,0)
+            case Var(v, _) => (0,0)
+            case Not(e) => 
+                var out := e.top_two_or_and_heights();
+                assert forall i :: i in this.children() ==> out.0 >= i.top_two_or_and_heights().0;
+                assert forall i :: i in this.children() ==>
+                    out.0 > i.top_two_or_and_heights().0 || out.1 >= i.top_two_or_and_heights().1;
+                out
+            case And(a,b) =>
+                assume false;
+                var out := merge_top_two(a.top_two_or_and_heights(), b.top_two_or_and_heights());
+                assert forall i :: i in this.children() ==> out.0 >= i.top_two_or_and_heights().0;
+                out
+            case Implies(a,b) =>
+                assume false;
+                var out := merge_top_two(a.top_two_or_and_heights(), b.top_two_or_and_heights());
+                assert forall i :: i in this.children() ==> out.0 >= i.top_two_or_and_heights().0;
+                out
+            case Equivalent(a,b) =>
+                assume false;
+                var out := merge_top_two(a.top_two_or_and_heights(), b.top_two_or_and_heights());
+                assert forall i :: i in this.children() ==> out.0 >= i.top_two_or_and_heights().0;
+                out
+            case Or(a,b) =>
+                assume false;
+                match (a,b) {
+                    case (And(_,_),And(_,_)) =>
+                        var out := (this.height(), this.height());
+                        assert forall i :: i in this.children() ==> out.0 >= i.top_two_or_and_heights().0;
+                        out
+                    case (a , And(_,_)) =>
+                        var out := merge_top_two(
+                            (this.height(), 0),
+                            merge_top_two(a.top_two_or_and_heights(), b.top_two_or_and_heights()));
+                        assert forall i :: i in this.children() ==> out.0 >= i.top_two_or_and_heights().0;
+                        out
+                    case (And(_,_) , b) =>
+                        var out := merge_top_two(
+                            (this.height(), 0),
+                            merge_top_two(a.top_two_or_and_heights(), b.top_two_or_and_heights()));
+                        assert forall i :: i in this.children() ==> out.0 >= i.top_two_or_and_heights().0;
+                        out
+                    case (a, b) =>
+                        var out := merge_top_two(a.top_two_or_and_heights(), b.top_two_or_and_heights());
+                        assert forall i :: i in this.children() ==> out.0 >= i.top_two_or_and_heights().0;
+                        out
+                }
+        }
     }
 
-    lemma DistributeEquivalent2(a: Expression, b: Expression, c: Expression, d: Expression, e: Expression, f: Expression)
-        requires a.Valid() && b.Valid() && c.Valid() && d.Valid() && e.Valid() && f.Valid()
-        requires a == And(c,d)
-        requires b == And(e,f)
-        ensures Or(a,b).equivalent(And(And(Or(c,e),Or(d,e)),And(Or(c,f),Or(d,f))))
+    predicate is_or_and()
     {
-        assert forall m: map<Variable, bool> :: true ==> 
-            (
-                ghost var vs: map<Variable, bool> :| vs == m;
-                var out := DistributeEquivalent2Abitrary(vs, a, b, c, d, e, f);
-                assert Or(a,b).eval(vs) == And(And(Or(c,e),Or(d,e)),And(Or(c,f),Or(d,f))).eval(vs);
-                Or(a,b).eval(m) == out.eval(m)
-            );
+        match this {
+            case Or(a,b) =>
+                match a {
+                    case And(_,_) => true
+                    case _ => false
+                }
+                || 
+                match b {
+                    case And(_,_) => true
+                    case _ => false
+                } 
+            case _ => false
+        }
     }
 
     predicate no_or_and()
     {
-        match this {
-            case Or(a,b) =>
-                match a {
-                    case And(_,_) => false
-                    case _ => true
-                }
-                && 
-                match b {
-                    case And(_,_) => false
-                    case _ => true
-                } 
-            case e => forall c :: c in e.children() ==> c.no_or_and()
-        }
+        !this.is_or_and() && forall c :: c in this.children() ==> c.no_or_and()
     }
 
-    function distribute_once() : (out: Expression)
-        requires this.Valid()
-        requires this.no_implies()
-        requires this.no_equivalent()
-        requires this.no_not()
-        requires match this {
-            case Or(a,b) => 
-                match a {
-                    case And(_,_) => true
-                    case _ => false
-                } && match b {
-                    case And(_,_) => false
-                    case _ => true
-                }
-                case _ => false
-        }
-        ensures out.Valid()
-        ensures out.no_implies()
-        ensures out.no_equivalent()
-        ensures out.no_not()
-        ensures this.equivalent(out)
-    {
-        match this {
-            case Or(a,b) =>
-                match (a,b) {
-                    case (a, And(bc1,bc2)) =>
-                        DistributeEquivalent(a,b,bc1,bc2);
-                        And(Or(a,bc1),Or(a,bc2))
-                    case _ => this
-                }
-            case _ => this
-        }
-    }
+    // ghost function or_and_heights() : (h: int)
+    //     ensures h >= 0
+    // {
+    //     (if this.is_or_and() then this.height() else 0)
+    //     +
+    //     match this {
+    //         case Constant(b) => 0
+    //         case Var(v, _) => 0
+    //         case Not(e) => e.or_and_heights()
+    //         case And(a,b) => a.or_and_heights() + b.or_and_heights()
+    //         case Or(a,b) => a.or_and_heights() + b.or_and_heights()
+    //         case Implies(a,b) => a.or_and_heights() + b.or_and_heights()
+    //         case Equivalent(a,b) => a.or_and_heights() + b.or_and_heights()
+    //     }
+    // }
+
+    // function distribute_one() : (out: Expression)
+    //     requires this.Valid()
+    //     requires match this {
+    //         case Or(a,b) =>
+    //             match a {
+    //                 case And(_,_) => false
+    //                 case _ => true
+    //             }
+    //             &&
+    //             match b {
+    //                 case And(_,_) => true
+    //                 case _ => false
+    //             } 
+    //         case _ => false
+    //     }
+    //     ensures out.Valid()
+    //     ensures this.equivalent(out)
+    //     ensures this.or_and_heights() > out.or_and_heights()
+    // {
+    //     match this {
+    //         case Or(a,b) =>
+    //             assert a.Valid() && b.Valid();
+    //             assert this.height() + a.or_and_heights() + b.or_and_heights() == this.or_and_heights();
+    //             assert a.height() < this.height();
+    //             assert b.height() < this.height();
+    //             match (a,b) {
+    //                 case (And(_,_),And(_,_)) => assert false; this
+    //                 case (a, And(bc1,bc2)) =>
+    //                     assert bc1.Valid() && bc2.Valid();
+    //                     assert b.or_and_heights() == bc1.or_and_heights() + bc2.or_and_heights();
+    //                     assert this.height() + a.or_and_heights() + bc1.or_and_heights() + bc2.or_and_heights() == this.or_and_heights();
+
+    //                     var or1 :=  Or(a,bc1);
+    //                     assert or1.or_and_heights() <= or1.height() + a.or_and_heights() + bc1.or_and_heights();
+    //                     assert or1.height() <= this.height();
+    //                     assert or1.or_and_heights() <= this.height() + a.or_and_heights() + bc1.or_and_heights();
+    //                     assert bc2.or_and_heights() >= 1;
+    //                     assert or1.or_and_heights() < this.height() + a.or_and_heights() + bc1.or_and_heights() + bc2.or_and_heights();
+    //                     assert or1.or_and_heights() < this.or_and_heights();
+
+    //                     var or2 :=  Or(a,bc2);
+
+    //                     var out := And(or1,or2);
+    //                     assert out.or_and_heights() == or1.or_and_heights() + or2.or_and_heights();
+    //                     out
+    //                 case _ => assert false; this
+    //             }
+    //         case _ => assert false; this
+    //     }
+    // }
 
     function distribute() : (out: Expression)
         requires this.Valid()
         requires this.no_implies()
         requires this.no_equivalent()
         requires this.no_not()
-        decreases this.height()
+        decreases this.height(), this.top_two_or_and_heights()
         ensures out.Valid()
         ensures out.no_implies()
         ensures out.no_equivalent()
         ensures out.no_not()
         ensures out.no_or_and()
         ensures this.equivalent(out)
+        ensures out.top_two_or_and_heights() == (0,0)
     {
         match this {              
             case Constant(_) => this
             case Var(_, _) => this
-            case And(a, b) => And(a.distribute(), b.distribute())
+            case And(a, b) => 
+
+                And(a.distribute(), b.distribute())
             case Or(a,b) =>
                 assert a.Valid() && a.no_implies() && a.no_equivalent() && a.no_not();
                 assert b.Valid() && b.no_implies() && b.no_equivalent() && b.no_not();
@@ -584,19 +685,28 @@ datatype Expression =
                         // var out := expanded.SubstituteChildren(and1, and2);
                         // assert this.equivalent(out);
                         this
-                    case (a, And(c,d)) =>
+                    case (a, And(e,f)) =>
                         assert {:split_here} true;
-                        DistributeEquivalent(b, a, c, d);
-                        var or1 := Or(a,c).SubstituteChildren(a, c.distribute());
+                        DistributeEquivalent(b, a, e, f);
+                        var e2 := e.distribute();
+                        assert e2.top_two_or_and_heights() == (0,0);
+                        var or1 := Or(a,e).SubstituteChildren(a, e2);
                         var or1 := or1.distribute();
-                        var or2 := Or(a,d).SubstituteChildren(a, d.distribute());
-                        var or2 := or2.distribute();
-                        var out := And(Or(a,c), Or(a,d)).SubstituteChildren(or1, or2);
-                        assert this.equivalent(out);
-                        assert out.no_or_and();
+
+                        assume false; 
+
+                        var f2 := f.distribute();
+                        var or2 := Or(a,f).SubstituteChildren(a, f2);
+                        var or2 := or2.distribute(); 
+
+                        var out := And(Or(a,e), Or(a,f)).SubstituteChildren(or1, or2);
+                        // assert out == And(or1, or2);
+                        // assert this.equivalent(out);
+                        // assert out.no_or_and();
                         out
                     case (And(c,d),b) =>
                         assert {:split_here} true;
+                        assume false; 
                         DistributeEquivalent(a, b, c, d);
                         var or1 := Or(b,c).SubstituteChildren(b, c.distribute());
                         var or2 := Or(b,d).SubstituteChildren(b, d.distribute());
@@ -612,29 +722,29 @@ datatype Expression =
         }
     }
 
-    function simplify() : (out: Expression)
-        requires Valid()
-        ensures out.Valid()
-        ensures out.no_implies()
-        ensures out.no_equivalent()
-        ensures out.no_not()
-        ensures out.no_or_and()
-        ensures this.equivalent(out)
-    {
-        var out := this;
-        var out := out.remove_implies();
-        var out := out.remove_equivalent();
-        var out := out.replace_not();
-        var out := out.distribute();
-        out
-    }
+    // function simplify() : (out: Expression)
+    //     requires Valid()
+    //     ensures out.Valid()
+    //     ensures out.no_implies()
+    //     ensures out.no_equivalent()
+    //     ensures out.no_not()
+    //     ensures out.no_or_and()
+    //     ensures this.equivalent(out)
+    // {
+    //     var out := this;
+    //     var out := out.remove_implies();
+    //     var out := out.remove_equivalent();
+    //     var out := out.replace_not();
+    //     var out := out.distribute();
+    //     out
+    // }
 
-    predicate no_and() {
-        match this {
-            case And(_,_) => false
-            case e => forall c :: c in e.children() ==> c.no_and()
-        }
-    }
+    // predicate no_and() {
+    //     match this {
+    //         case And(_,_) => false
+    //         case e => forall c :: c in e.children() ==> c.no_and()
+    //     }
+    // }
 
     // function make_clause() : (c : Clause)
     //     requires Valid()
